src/ref4/Curve25519_ref4.ec
@@ -6,8 +6,6 @@ import SLH64.
 require import Array4 Array5 Array8 Array32.
 require import WArray32 WArray40 WArray64.
 
-
-
 module M = {
   proc __load4 (p:W64.t) : W64.t Array4.t = {
     var aux: int;
